Dafny fixes (#2884)
* Fix for uninitialized variables.

After adding the predicate RecordedCheckpointsRecvdCameFromNetwork
to the invariant we found omitted variables in the Init predicate.

* Fix for SendPrePrepare to use PrePrepare's constructor.

We use the correct Message constructor to avoid errors when
specifying the PrePrepare message that will be sent.

docs/sbft-formal-model/proof.dfy
@@ -43,7 +43,7 @@ module Proof {
               && var replicaVariables := v.hosts[replicaIdx].replicaVariables;
               && var replicaConstants := c.hosts[replicaIdx].replicaConstants;
               && seqID in replicaVariables.workingWindow.getActiveSequenceIDs(replicaConstants)
-              && replicaVariables.workingWindow.prePreparesRcvd[seqID].Some? 
+              && replicaVariables.workingWindow.prePreparesRcvd[seqID].Some?
                 :: v.hosts[replicaIdx].replicaVariables.workingWindow.prePreparesRcvd[seqID].value in v.network.sentMsgs)
   }
 
@@ -260,6 +260,16 @@ module Proof {
                         == prepare.payload.operationWrapper)
   }
 
+  predicate RecordedCheckpointsRecvdCameFromNetwork(c:Constants, v:Variables) {
+    && v.WF(c)
+    && (forall replicaIdx, checkpointMsg | 
+              && IsHonestReplica(c, replicaIdx)
+              && var replicaVariables := v.hosts[replicaIdx].replicaVariables;
+              && var replicaConstants := c.hosts[replicaIdx].replicaConstants;
+              && checkpointMsg in replicaVariables.checkpointMsgsRecvd.msgs
+                :: checkpointMsg in v.network.sentMsgs)
+  }
+
   // predicate PrePreparesCarrySameClientOpsForGivenSeqID(c:Constants, v:Variables)
   // {
   //   && v.WF(c)
@@ -299,6 +309,7 @@ module Proof {
     && HonestReplicasLockOnPrepareForGivenView(c, v)
     && HonestReplicasLockOnCommitForGivenView(c, v)
     && CommitMsgsFromHonestSendersAgree(c, v)
+    && RecordedCheckpointsRecvdCameFromNetwork(c, v)
   }
 
   function sentPreparesForSeqID(c: Constants, v:Variables, view:nat, seqID:Messages.SequenceID,
@@ -615,7 +626,7 @@ module Proof {
     && var h_v' := v'.hosts[step.id].replicaVariables;
     && Replica.NextStep(h_c, h_v, h_v', step.msgOps, h_step)
     && h_step.SendPrePrepareStep?
-    && Replica.SendPrePrepare(h_c, h_v, h_v', step.msgOps)
+    && Replica.SendPrePrepare(h_c, h_v, h_v', step.msgOps, h_step.seqID)
   }
 
   lemma SendPrePrepareStepPreservesInv(c: Constants, v:Variables, v':Variables, 
@@ -995,7 +1006,7 @@ module Proof {
       //QuorumOfPreparesInNetworkMonotonic(c, v, v', step, h_step); // not part of the proof yet
       
       match h_step
-        case SendPrePrepareStep() => {
+        case SendPrePrepareStep(seqID) => {
           SendPrePrepareStepPreservesInv(c, v, v', step, h_step);
         }
         case RecvPrePrepareStep() => {
